
\chapter{Introduction to Mean curvature flow}

\section{Fundamentals of Hypersurfaces}
SET UP THE FOLLOWING  - 

1. SECOND FUNDAMENTAL FORM\\
2. MEAN CURVATURE\\
3. CONVEXITY RESULTS\\
4. MCF AS GRADIENT FLOW OF AREA\\
5. CODAZZI IDENTITY, SIMONS IDENTITY\\
6. UMBILLIC HYPERSURFACES ARE SPHERES\\


Let $M^{n}$ be a smooth $ n $-dimensional manifold with a smooth immersion $ X : M^{n} \to \R^{n+1} $. If $ X $ is a diffeomorphism onto its image, we say $ X $ is an embedding and its image $ \mathcal{M}^{n} = X(M^{n}) $ has the structure of a smooth $ n $-dimensional submanifold of $ \R^{n+1} $. Let $ (U, \{x^{i}\}) $ be a coordinate system on $ M^{m} $, in Euclidean coordinates the pushforward of tangent vectors will be 
    \[ dX( \partial_{i}) \define \frac{ \partial X}{ \partial x^{i}} = \partial_{i}X \]
where $ dX : TM^{n} \to T\R^{n+1} $ is the derivative of $ X $. Since $ dX $ is an injection for each point in $ M^{n} $, we can define an inner product on $ T(M^{n}) $ which in local coordinates is given by 
    \[ g( \partial_{i}, \partial_{j}) = \left< \partial_{i}X, \partial_{j}X \right> \]
where $ \left< \cdot, \cdot \right> $ denotes the standard inner product on Euclidean space. 
Further we can define the Levi-Civita connection on $ M^{n} $ from the Levi-Civita connection on $ \R^{n+1} $. The Levi-Civita connection on $ \R^{n+1} $ is given by 
\[ D_{X}Y =  X(Y^{i}) \partial_{i}\] (TO DO)
Let $ x \in M^{n} $ and $ u \in T_{p}M^{n}, \tilde{v} \in T|_{U}M^{n}$ for some open set $ U $ containing $ x $. Define a connection $ \nabla $ by 
\begin{equation}
    dX(\nabla_{u}\tilde{v}) = D_{dX(u)}(\tilde{V}) \label{connection}
\end{equation}
where $ \tilde{V} $ is an extension of $ dX(\tilde{v}) $ to an open set of $ \Rn $ containing $ X(U) $. 
\begin{thm}
    The connection defined by \cref{connection} is well-defined and is the unique Levi-Civita connection on $ (M^{n},g) $
\end{thm}
When $ X $ is an embedding, the restriction of the tangent bundle of $ T\Rn|_{\mathcal{M}^{n}} $ can be decomposed as the direct sum 
\[ T\mathcal{M}^{n}\oplus N\mathcal{M}^{n}  \]
where $ N\mathcal{M}^{n} $ is the normal bundle which can be described as 
\[ N\mathcal{M}^{n} = \{(p,\nu) \in T\Rn|_{ \mathcal{M}} : \left< u, \nu \right> =0 \text{ for all } u \in T_{p} \mathcal{M}\} \]

\section{Evolution equations}
Let $X : M^n \times I \to \R^{n+1}$ be a smooth $1$-parameter family of immersions such that 

\[ \dou_t X(p,t) = \overrightarrow{H}(x,t)  = -H(x,t)\nu(x,t)\]

Let $\{x^i\}$ be a local coordinate in $M^n$. Then the induced metric on the hypersurface is given by $g = X^*(\delta)$ where $\delta$ is the flat metric on $\R^{n+1}$. This gives
\[ g_{ij} = \delta(X_*(\dou_i),X_*(\dou_j)) = \left\langle  \frac{\dou X}{\dou x^i}, \frac{\dou X}{\dou x^j} \right\rangle  \]
\begin{thm} Let $X: M^n \times I \to \R^{n+1}$ be a solution of mean curvature flow. Then the evolution equation of metric, normal, second fundamental form, mean curvature is given by
\begin{equation}
    \dou_t g_{ij} = -2Hh_{ij}
\end{equation}
\begin{equation}
\dou_t \nu  = \nabla H
\end{equation}
\begin{equation}
\dou_t h_{ij} = \Delta h_{ij} - 2Hh_{il}g^{lm}h_{mj}+|A|^2h_{ij}
\end{equation}
\begin{equation}
    \dou_t H = \Delta H + |A|^2H
\end{equation}
\end{thm}
\begin{proof}
1. In local coordinates we have 
\begin{align*}
    \dou_tg_{ij} & = \frac{\dou}{\dou t} \left\langle \frac{\dou X}{\dou x^i}, \frac{\dou X}{\dou x^j} \right\rangle \\
& = \left\langle \frac{\dou^2X}{\dou x^i \dou t}, \frac{\dou X}{\dou x^j} \right\rangle + \left\langle \frac{\dou X}{\dou x^i}, \frac{\dou^2 X}{\dou t \dou x^j} \right\rangle\\
& = \left\langle \frac{\dou}{\dou t}(-H\nu), \frac{\dou X}{\dou x^j} \right\rangle + \left\langle \frac{\dou X}{\dou x^i}, \frac{\dou }{\dou x^j}(-H\nu)\right\rangle \\
& = -H \left\langle \frac{\dou \nu}{\dou t}, \frac{\dou X}{\dou x^j}\right\rangle  - H \left\langle \frac{\dou X}{\dou x^i}, \frac{\dou \nu}{\dou t}\right\rangle \\
& = -2Hh_{ij}
\end{align*}
2. Since $\langle \nu, \nu \rangle = 1$, we have $2\langle \frac{\dou \nu}{\dou t}, \nu \rangle = 0$, so the vector $\frac{\dou \nu}{\dou t}$ is in the tangent plane of the hypersurface, hence we can write it as a linear combination of $\{\frac{\dou X}{\dou x^j}\}$ to get
\begin{align*}
\frac{\dou \nu}{\dou t} &= \left\langle \frac{\dou \nu}{\dou t}, \frac{\dou X}{\dou x^i} \right\rangle \frac{\dou X}{\dou X^j}g^{ij} = - \left\langle \nu, \frac{\dou }{\dou x^i}\left( \frac{\dou X}{\dou t}\right) \right\rangle\frac{\dou X}{\dou x^j}g^{ij} \\
& = \left\langle \nu, \frac{\dou }{\dou x^i}\left( H \nu \right) \right\rangle \frac{\dou X}{\dou x^j}g^{ij}\\
& = \frac{\dou H}{\dou x^i}\frac{\dou X}{\dou x^j}g^{ij} + H \left\langle \nu, \frac{\dou \nu}{\dou x^i}\right\rangle \frac{\dou X}{\dou x^j}g^{ij}\\
& = \frac{\dou H}{\dou x^i}\frac{\dou X}{\dou x^j}g^{ij} = \nabla H
\end{align*}
3. From the relation \[
\frac{\dou^2 X}{\dou x^{i} \dou x^{j}} = \Gamma^{k}_{ij}\frac{\dou X}{\dou x^{k}}	
,\] we get 
\begin{align*}
\dt h_{ij} & = - \dt (\frac{\dou^2 X}{\dou x^i \dou x^j},\nu)\\
& = (\frac{\dou^2}{\dou x^i \dou x^j}(H \nu), \nu) - 
.\end{align*}
4. From the previous equation we get 
\begin{align*}
\dou_t H &= \dou_t(g^{ij}h_{ij}) = \frac{\dou g^{ij}}{\dou t}h_{ij}+ g^{ij}\frac{\dou h_{ij}}{\dou t}\\
& = -g^{ik}\frac{\dou g_{kl}}{\dou t}g^{lj}h_{ij}+ g^{ij}(\Delta h_{ij} - 2Hh_{il}g^{lm}h_{mj}+|A|^2h_{ij})\\
& = -g^{ik}(-2Hh_{kl})g^{lj}h_{ij}+ \Delta(g^{ij}h_{ij}) - 2Hg^{ij}g^{lm}h_{il}h_{mj}+|A|^2H\\
& = 2H|A|^2 + \Delta H - 2H|A|^2 + |A|^2H\\
& =  \Delta H+ |A|^2H
\end{align*}
\end{proof}
\begin{corollary}
If mean curvature is positive everywhere on the initial hypersurface, then it remains so throughout the flow.
\end{corollary}
\begin{proof}
We apply maximum principle to the evolution equation of $H$.
\end{proof}
\begin{remark}
This property of mean curvature holds even when the hypersurface is embedded in an arbitrary(OR WITH POSITIVE RICCI CURVATURE?) Riemannian manifold. 
\end{remark}
\section{The Avoidance Principle}

Let $X_i : M^n_i \times  [0,T) \to \R^{n+1}, i = 1,2 $ be properly immersed solutions to mean curvature flow such that at least one of  $ M^n_1$ or $M^n_2$ is compact. 
If the hypersurfaces are disjoint initially, i.e. $X_1(M^{n_1},0)\cap X_2(M^n_2,0) = \phi$, then they remain so. Define the distance function $d: M^n_1 \times M^n_2 \times  [0,T) \to \R$ between the solutions by \[
d(x,y,t) = |X_2(y,t) - X_1(y,t)|
.\] 
as a function of time. From the assumption of compactness $d_0 \define \inf_{(x,y) \in M^n_1 \times M^n_2} d(x,y,0) >0$
\begin{figure}[h]
\centering
\begin{tikzpicture}
    \draw [red] plot [smooth cycle] coordinates {(3,0)(0,3)(-3,0)(0,-3)};
    %\draw [red](0,0) circle (3cm);
    \fill [red!20] plot [smooth cycle] coordinates {(3,0)(0,3)(-3,0)(0,-3)};
    
    
    \draw [green] plot [smooth cycle] coordinates {(2.5,0)(0,2.5)(-2.5,0)(0,-2.5)};
    \fill [green!20] plot [smooth cycle] coordinates {(2.5,0)(0,2.5)(-2.5,0)(0,-2.5)};
    \draw [dashed,green] (2.5,0) arc (60:120:5cm);
    \draw [green] (-2.5,0) arc (240:300:5cm);
    \draw [thick,green][-stealth](2.75,0) -- (2,0);
    \draw [thick,red][-stealth](3,0) -- (2.5,0);
    \draw [dashed,red] (3,0) arc (60:120:6cm);
    \draw [red] (-3,0) arc (240:300:6cm); 
\end{tikzpicture}
\caption{Disjoint hypersurfaces flowing under MCF}
\end{figure}
\begin{thm}
If $X_1$ and $X_2$ are solutions to mean curvature flow on closed manifolds with $ d_{0}>0$, then $ d(x,y,t)>0$ for all $ x,y,t$. In particular, if $ X_1(x,0) \neq X_2(y,0)$ for all $x \in M^n_1  $ and $ y \in M^n_2$, then $ X_1(x,t) \neq X_2(y,t)$ for all $ x \in M^{n}_1$, $y \in  M^n_2$ and $ t \in  [0,T)$. 
\end{thm}
\begin{proof}
Assume on the contrary $ d(x,y,t)$ is not everywhere strictly greater that $ d_{0} $. Then there exists a $ t_{0} $ such that $ d(x_{0},y_{0},t_{0}) = d_{0} - \delta $
\end{proof}
\begin{remark}
From the proof we can conclude that the distance between the hypersurfaces is a non-decreasing function. Another way to see this is that $ d_{t} $ satisfies a heat-type parabolic equation 
    \[ TO\, DO \]
 on which maximum principle is applicable. 
\end{remark}
\begin{proof} Fix $\epsilon > 0$ and suppose that $e ^{\epsilon (1+t)}d(x,y,t)$ is not strictly greater than $d_0$. That is there exists a time $ t_0 > 0$ such that $e^{\epsilon(1+ t)}d(\cdot, \cdot, t)$ reaches $ d_0$. That is,\[
e^{\epsilon(1+t)}d(\cdot,\cdot,t)> 0 \quad \text{ for } t < t_0
.\]  and \[
e^{\epsilon(1+t)}d(x_0,y_0,t_0) = d_0 \quad \text{ for some }(x_0,y_0) \in   M^n_1 \times  M^n_2		
.\] Then \[
\pt (e^{\epsilon(1+t)}d)|_{(x_0,y_0,z_0)} \le 0 
.\] Let $D$ denote the Euclidean directional derivative, by $ \nabla_i$ the covariant derivative induced on $M^n_i$ by $X_i$, and by $\nabla $ the covariant derivative on $ M^n_1 \times  M^n_2$ induced by $ \nabla_1$ and $ \nabla_2$, we find \[
\nabla^2
.\] 

\end{proof}
\begin{remark}
We can phrase the avoidance principle as : disjointness is an immortal property and jointness is an ancient property.
\end{remark}

\section{Huisken's theorem}

Huisken's theorem proves the convergence of compact, uniformly convex hypersurface to sphere under Mean curvature flow in finite time. 
\begin{thm}
Let $ X : M^{n} \times [0,T) \to \Rn  $, $ n \ge 2 $ be a maximal solution of MCF such that $ M^{n} $ is compact and $X_{0} = X(\cdot, 0)$ is convex embedding. Then $ X_{t} = X(\cdot,t) $ is a convex embedding for all $ t>0 $ and $ X_{t} $ converges to a point $ p \in \Rn $ as $ t \to T $. Further the rescaled embeddings $ \tilde{X}_{t} : M^{n} \to \Rn $ defined by 
            \[ \tilde{X}_{t}(x) \define \frac{X_{t}(x)-p}{\sqrt{2n(T-t)}}\]
converge uniformly in the smooth topology to a smooth embedding whose image coincides with the unit sphere $ S^{n} $.
\end{thm}
\subsection{Long time existence}

In this subsection we will prove that blowing up of second fundamental form is the only obstruction for continuing the flow. The proof goes by contradiction, relying on the Bernstein type estimates. This technique is very similar to the one Hamilton used for Ricci flow \cite{hamilton1982three}.

\begin{thm}
    Let $ X : M^{n} \times [0,T) \to \Rn $ be a solution of the mean curvature flow with $ M^{n} $ compact. If $ X $ is maximal then $ T< \infty $ and 
    \[ \sup_{M^{n} \times [0,T)} |A| = \infty.\]
\end{thm}
\begin{proof}
    Assume on the contrary that $ \sup_{M^{n} \times [0,T)}|A|^{2} \le C $. Our aim is to prove that the manifold $X(\cdot, t)= \mathcal{M}_{t} $ converges to a smooth limit $ \mathcal{M}_{T} $ as $ t \to T $ which will give a contradiction by applying short time existence of mean curvature flow.
\end{proof}
\subsection{Pinching estimate}

The quantity $ \frac{|A|^{2} - \frac{H^{2}}{n}}{H^{2}} = \frac{1}{n} \sum_{i<j}^{} \left( \frac{\kappa_{i}}{H}- \frac{\kappa_{j}}{H} \right)^{2}  $ is scaling invariant and measures the roundness of the hypersurface. If we compute the evolution equation we get \begin{equation}
EQUATION
\end{equation} 
but the maximum principle is not directly applicable because of the positive last term. So we do not directly get a pointwise $ L^{\infty} $ bound we do the next best thing possible which is $ L^{p} $ bounds. After obtaining this there is a sophisticated iteration argument developed by Stampacchia which allows us to produce an $ L^{\infty} $ estimate. See  \href{https://youtu.be/a577KPiOoxw?t=1790}{here}
\begin{thm}
There exists constants $ \delta $ and $ C_{0} < \infty $ depending only on $ \mathcal{M}_{0} $ such that 
\[ |A|^{2} - \frac{H^{2}}{n} \le C_{0}H^{2-\delta} \]
for $ t \in (0,T] $.

\end{thm}
Let $ f_{\sigma} = \frac{|A|^{2}- \frac{H^{2}}{n}}{H^{2-\sigma}} = \left(\frac{|A|^{2} - \frac{H^{2}}{n}}{H^{2}}\right)H^{\sigma}$, then the evolution equation of $ f_{\sigma} $ is 
\begin{lemma}
The evolution of $ f_{\sigma} $ is given by \begin{align*}
    \frac{ \partial}{ \partial t}f_{\sigma} & = 
\end{align*}
\end{lemma}
(Huisken' remark on this from the lecture series : the bad term can only be controlled using integral estimates \href{https://www.mfo.de/about-the-institute/staff/prof-dr-gerhard-huisken/lectures/mean-curvature-flow/lecture-3}{58 min mark} )

(Sinestrari intuition about Stampacchia iteration : \href{https://youtu.be/XvUGowx9WNo?t=2119}{yt link})

\subsection{Width-pinching}

Let $ \Omega  \subset \Rn  $ be a compact, convex body with  boundary $  \mathcal{M}  = \partial \Omega$. %such that $ \mathcal{M} $ is locally uniformly convex. 
%This allows us to define inverse of the Gauss map on the hypersurface $ \mathcal{M} $. 
Define the support function $ \sigma : S^{n} \to \R $ as follows 
\[ \sigma(z) \define \sup_{x \in \Omega}\left< x,z \right> .\]
Using this we define the width function of $ \Omega $ by 
\[ w(z) = \sigma(z)+ \sigma(-z) \qquad \text{ for all } z \in S^{n} \]
which as the name suggests measures the width of $ \Omega  $ in the direction $ z$. Let $ w_{+} $ and $ w_{-} $ denote the maximum and minimum width. It is easy to see that maximum width is the diameter of $ \Omega $, so 
\[ w_{+} = \sup_{x,y \in \Omega}||x-y||. \]
If $ \mathcal{M}$ is smooth uniformly convex hypersurface, then we can write the support function in terms of Gauss map $ G : \partial \Omega \to S^{n} $ as 
\[ \sigma(z) = \left< G^{-1}(z), z \right>, \] so 
\[ \sigma(G(z)) = \left< z,G(z) \right>.\]

It is a lemma by Andrews that the pinching of principal curvatures implies the pinching of the widths, which will be later important to prove convergence of the hypersurface into a point. 
\begin{lemma}
Let $ \Omega \subset \Rn $, $ n \ge 2 $ be a uniformly convex body with compact, smooth boundary $ \mathcal{M} = \partial \Omega $. Suppose the principal curvatures of $ \mathcal{M} $ are pinched by a constant $ C < \infty $, i.e. $ \kappa_{n}(x) \le C \kappa_{1}(x) $ for all $ x \in \mathcal{M}  $. Then the widths of $ \mathcal{M} $ are pinched by the same constant, so 
\[ w_{+} \le C w_{-} \]
\end{lemma}
\begin{proof}
We will first prove it for $ n=2 $, which presents the main idea. Let $ e  \in S^{2}$ be unit vector in $ \R^{3} $ and (TO DO LATER) 
\end{proof}

We know the solution of MCF of spheres, so it will be useful to relate the widths of the hypersurface to the spheres inscribed and circumscribed about it. Let $$ \rho_{+} \define \inf\{r : \Omega \subset B_{r}(x) \text{ for some }x \in \R^{n}\}$$ denote the circumradius and 
\[ \rho_{-} \define \sup\{B_{r}(X) \subset \Omega \text{ for some }x \in \R^{n}\} \]
denote the inradius radius. There is also a relation between inscribed and circumscribed radius to widths of the hypersurface as given by the following lemma
\begin{lemma}
On any bounded convex body $ \Omega \subset \Rn $, 
\[ \rho_{+} \le \sqrt{n+1}w_{+} \quad \text{ and } \quad \rho_{-} \ge \frac{1}{n+2}w_{-}.\]
\end{lemma}
\begin{remark}
These are not the best bounds however they are sufficient for our purpose.
\end{remark}

Combining the two lemmas, we get 
\begin{equation}
\rho_{+} \le \frac{n+2}{\sqrt{n+1}}C\rho_{-} \label{pinching}
\end{equation}

Let $ \{\mathcal{M}_{t}\}_{t \in [0,T)}$ be family of hypersurfaces flowing under MCF with maximal time $ T $ and the initial pinching constant given by
\[ C = \sup_{ \mathcal{M}_{0}} \frac{\kappa_{n}}{\kappa_{1}} \]

If we can show that $ \rho_{-} \to 0 $ as $ t \to T $, then inequality (\ref{pinching}) would imply $ \rho_{+} \to 0 $. This proves the convergence of hypersurfaces to a point. 
\begin{thm}
The inradius $ \rho_{t} $ of $ \Omega_{t} $ tends to zero as $ t \to T $. Thus, $ \mathcal{M}_{t} $ converges to some point $ p \in \Rn $ as $ t \to T $.
\end{thm}

\section{Monotonicity Formula}
Let $ X :M^{n} \times I \to \R^{n+1} $ be one-parameter family of immersions flowing by mean curvature. Let $ \{x^{i}\} $ be local coordinates around a point $ p \in M $. Then the metric and second fundamental form are given by 
\[ g_{ij} = \left< \frac{\dou X}{\dou x^{i}}, \frac{\dou X}{\dou x^{j}} \right> , \qquad h_{ij} = \left<\eta, \frac{\partial^{2}X}{\dou x^{i}\dou x^{j}} \right> \]

If we scale the solution by a factor of $ \lambda  $, defined by $ \tilde{X}(x,t) = \lambda X(x,t) $ we get the following metric and second fundamental form 

\[ \tilde{g_{ij}} = \left< \frac{\dou \tilde{X}}{\dou x^{i}}, \frac{\dou \tilde{X}}{\dou x^{j}} \right>  = \lambda^{2}g_{ij} \]
\[ \tilde{h_{ij}} = \left<\eta, \frac{\partial^{2}\tilde{X}}{\dou x^{i}\dou x^{j}} \right>  = \lambda h_{ij}\]

so the scaled mean curvature is given by $ \tilde{H} = \tilde{g}^{{ij}}\tilde{h}_{ij} = \frac{1}{\lambda}H $. This implies the scaled solutions satisfy the evolution equation

\[ \frac{\dou \tilde{X}}{\dou t} = \lambda \frac{\dou X}{\dou t} = -\lambda^{2}\tilde{H}\eta \]

    \[ \frac{\dou \tilde{X}}{\dou (\lambda^{2}t)} = - \tilde{H}\eta \]
Hence if scale time by $ \lambda^{2} $, then $ \tilde{X} $ is also a solution of the MCF. 

Mean curvature flow is invariant under parabolic scaling, i.e.  if $ X : M^{n} \times I \to \R^{n+1} $ is solution, then so is $ X_{\lambda}(x,t) = \lambda X(x,\lambda^{2}t) $. We construct a weighted area functional which is invariant under \textit{parabolic} scaling along any solution to mean curvature flow which will be monotonous.

Let $ \rho(x,t) $ be the backward heat kernel at $ (X_{0},t_{0}) $, i.e.,   \[\rho(x,t) = \frac{1}{(4 \pi (t_{0}-t))^{ \frac{n}{2}} }\cdot \exp\left( - \frac{|X(x,t)-X_{0}|^{2}}{4(t_{0}-t)} \right), \qquad t<t_{0} \]
\begin{thm}
If $ M_{t} $ is a solution of mean curvature flow for $ t< t_{0} $, then we have the formula

    \[ \frac{d}{dt} \int_{M_{t}}\rho(x,t)d \mu_{t}  = - \int_{M_{t}}\rho(x,t)\left( H- \frac{\left< X(x,t)-X_{0}, \eta \right>}{2 (t_{0}-t)} \right)^{2}d \mu_{t}\] 

\end{thm}
\begin{proof}
To simplify the formula assume that $ \left(X_{0},t_{0}\right) = (0,0) $. We know that $ \frac{d}{dt} \mu_{t} = -H^{2} \mu_{t} $, so differentiating $ \rho $ with respect to time we get,
\begin{align}
    \frac{d}{dt} \int_{M_{t}}\rho(x,t)d \mu_{t}  &= \int_{M_{t}}\rho(x,t)(-H^{2})d \mu_{t} + \int_{M_{t}} \frac{\dou}{\dou t}\rho(x,t)d \mu_{t}\nonumber \\
    & = -\int_{M_{t}}\rho(x,t)H^{2}d \mu_{t} +\int_{M_{t}}\left( \frac{\left< X(x,t), H(x,t)\eta \right>}{2(-t)}\rho(x,t) \right)d\mu_{t}\nonumber \\
    &  \qquad \qquad  + \int_{M_{t}} \left( \frac{n}{2(4 \pi)(-t)}(4 \pi)\rho(x,t) -\frac{|X(x,t)|^{2}}{4(-t)^{2}}\rho(x,t)\right)d \mu_{t}\nonumber \\ 
    & = \int_{M_{t}}\rho\left(   \frac{n}{2(-t)} +\frac{\left< X,H \eta\right>}{2(-t)}- \frac{|X|^{2}}{4(-t)^{2}} -H^{2}\right)d \mu_{t}\label{rho0}
    %& = -\int_{M_{t}}\rho \left| H \eta + \frac{X}{2(-t)}\right|^{2}d \mu_{t} + \int_{M_{t}}\rho \frac{ \left< X,H \eta \right>}{2(-t)} d \mu_{t} + \int_{M_{t}} \frac{n\rho}{2(-t)}d \mu_{t} \label
\end{align}

Now $ \Delta X = - H \eta $, using this relation for second term and divergence theorem we get 
\begin{align}
\int_{M_{t}}\rho \left< X,H \eta \right> d \mu_{t} & =  -\int_{M_{t}} \rho\left< X,\Delta X \right> d \mu_{t} \nonumber \\ 
& = - \sum_{k=1}^{n+1}\int_{M_{t}} \rho X_{k} \Delta X_{k} d \mu_{t}\nonumber \\
& = \sum_{k=1}^{n+1} \int_{M_{t}} \left< \nabla(\rho X_{k}), \nabla X_{k} \right>d \mu_{t}\nonumber \\ 
& = \sum_{k=1}^{n+1} \int_{M_{t}} \left( \left< \nabla\rho, \nabla X_{k} \right>X_{k} + \rho \left< \nabla X_{k}, \nabla X_{k} \right> \right)d \mu_{t} \label{rho1}
% & = \int_{M_{t}} \left< \nabla(\rho X), \nabla X \right>d \mu_{t}\\ 
% & = \int_{M_{t}} \left( \rho\left< \nabla X, \nabla X  \right> + \left< \nabla \rho, \nabla X \right> X \right)
\end{align}
Let $ (U,\{x^{i}\}) $ be some local coordinates on the hypersurface. In these coordinates we can write $ \nabla \rho = g^{ij} \partial_{i} \rho \partial_{j} $, so $  \left< \nabla \rho , \nabla X_{k}\right> = \nabla \rho (X_{k}) = g^{ij} (\partial_{i}\rho) (\partial_{j}X_{k}) $ which implies 
\begin{align}
\sum_{k=1}^{n+1} \left< \nabla \rho , \nabla X_{k}  \right> X_{k} & = \sum_{k=1}^{n+1}  g^{ij} (\partial_{i}\rho) (\partial_{j}X_{k}) X_{k}\nonumber \\ 
& = g^{ij}( \dou_i \rho) \left< X, \dou_j X \right>\nonumber \\
& = g^{ij} \rho \left( \frac{-\left< X, \partial_{i}X \right>}{2(-t)} \right) \left< X, \dou_j X \right>\nonumber \\
& = - \frac{\rho}{2(-t)}|X^T|^2 \label{rho2}
\end{align}
and 
\begin{equation}
\sum_{k=1}^{n+1} \rho  \left< \nabla X_{k}, \nabla X_{k} \right> = \sum_{k=1}^{n+1} \rho g^{ij} (\partial_{i} X_{k} )(\partial_{j}X_{k}) = \rho g^{ij} \left<  \partial_{i}X, \partial_{j}X \right> = \rho g^{ij}g_{ij} = n \rho \label{rho3}
\end{equation}
Substituting \cref{rho2} and \cref{rho3} into \cref{rho1} and multiplying by $ \frac{1}{2(-t)} $, we get 
\begin{equation*}
\int_{M_{t}}\rho  \frac{\left< X,H \eta \right>}{2(-t)} d \mu_{t}  = \int_{M_{t}} \rho \left( \frac{n}{2(-t)} - \frac{1}{4(-t)^2}|X^T|^2  \right) d \mu_{t} 
\end{equation*}
or 
\begin{equation}
\int_{M_{t}}\frac{n\rho}{2(-t)} d \mu_{t} = \int_{M_{t}} \rho \left(  \frac{\left< X,H \eta \right>}{2(-t)} + \frac{1}{4(-t)^2}|X^T|^2 \right)d \mu_{t}\label{rho4}
\end{equation}
where $ X^{T} $ denotes the tangential part of the vector $ X $. Substituting \cref{rho4} into \cref{rho0}
\begin{align*}
\frac{d}{dt} \int_{M_{t}}\rho(x,t)d \mu_{t}  &=  \int_{M_{t}}\rho\left(\frac{\left< X,H \eta\right>}{(-t)}- \frac{|X|^{2}}{4(-t)^{2}} -H^{2}+ \frac{1}{4(-t)^2}|X^T|^2\right)d \mu_{t}\\ 
& = -\int_{M_{t}} \rho \left( H - \frac{\left< X, \eta \right>}{2(-t)} \right)^{2} d \mu_{t}
\end{align*}
\end{proof}

\subsection{Rescaled Monotonicity formula}

From section (?) we know that the curvature blows up at the maximal time $ T $  and satisfies the inequality

\[ \max_{p \in M}|A(p,t)| \ge \frac{1}{\sqrt{2(T-t)}} \]

\begin{defn}
Let $ T $ be the maximal time of existence of a mean curvature flow. If there exists a constant $ C >1 $ such that 

    \[ \max_{p \in M}|A(p,t)| \le \frac{C}{\sqrt{2(T-t)}} \]
we say the flow is developing at time $ T $ a \textit{type I singularity}.
\end{defn}

Conversely, if such a constant does not exist, that is 

\[ \limsup_{t \to T} \max_{p \in M}|A(p,t)|\sqrt{T-t} = \infty \]

we say that we have a \textit{type II singularity}. We will restrict ourselves to type I singularity for the rest of this section. 


\section{Surfaces of positive mean curvature}

From the maximum principle we know that if mean curvature of the initial hypersurface $M_0$ is positive then it will stay positive on $M_t$. 
For self-similar solutions, we know that the limiting hypersurface will satisfy the equation $H = \langle x, \nu \rangle$. 
We prove that sphere is the only compact hypersurface of positive mean curvature moving under self-similarity 
\begin{thm}
If $M^n$, $n\ge 2$, is compact with non-negative mean curvature $H$ and satisfies the equation $H = - \langle X, \nu \rangle$, then $M^n$ is a sphere of radius $\sqrt{n}$. 
\end{thm}
\begin{proof}
Suppose the hypersurface satisfies $H = -\langle X, \nu \rangle$. Let $e_1,\ldots, e_n$ be an orthonormal frame on $M^n$, then 
\begin{align}
    \nabla_{i}H & = - \left< D_{e_{i}}X, \nu \right> - \left< X, \nabla_{e_{i}}\nu \right> \nonumber \\
    & = -\left< e_{i}, \nu \right> - \left< X, \left< \nabla_{e_{i}}\nu,e_{l} \right>e_{l} \right>\nonumber \\ 
    & = \left< X,e_{l} \right>h_{il}
\end{align}
\[\nabla_i \nabla_j H = h_{ij} - Hh_{il}h_{lj}+\langle x, e_l \rangle \nabla_l h_{ij}\]
\end{proof}

\section{Maximum principle}\label{max}
We can extend the maximum principle on Euclidean space to general Riemannian manifolds. 
\begin{lemma}
Let 
\end{lemma}